FTA up to some nonsense about boolean type conversions

definitions.lean
@@ -42,14 +42,43 @@ def product : list ℕ → ℕ
 | []       := 1
 | (h :: t) := h * (product t)
 
+-- helpful to work with max instead of min: what is min of []?
 def lmax : list ℕ → ℕ
-| []       := 0
-| (h :: t) := max h (lmax t)
+| []        := 0
+| (h :: t)  := max h (lmax t)
 
 def sorted : list ℕ → bool
-| []       := tt
-| (h :: t) := (max h (lmax t) = h) ∧ sorted t
+| []        := tt
+| (h :: t)  := (max h (lmax t) = h) ∧ sorted t
 
 def plist : list ℕ → Prop
 | []       := tt
 | (h :: t) := number_theory.irreducible h ∧ plist t
+
+namespace list
+
+/-
+The following definitions for permutations and insertion sort are ripped from
+mathlib. But I wrote my own proofs about these objects (in list_extra.lean)
+because I didn't like the ones in mathlib (they generally seemed a bit obscure
+and they rope in a lot of machinery e.g. set theory that I don't want to
+talk about).
+-/
+
+inductive perm {α : Type} : list α → list α → Prop
+| nil   : perm [] []
+| skip  : Π (x : α) {l₁ l₂ : list α}, perm l₁ l₂ → perm (x::l₁) (x::l₂)
+| swap  : Π (x y : α) (l : list α), perm (y::x::l) (x::y::l)
+| trans : Π {l₁ l₂ l₃ : list α}, perm l₁ l₂ → perm l₂ l₃ → perm l₁ l₃
+
+infix ~ := perm
+
+@[simp] def ordered_insert (a : ℕ) : list ℕ → list ℕ
+| []       := [a]
+| (b :: l) := if b ≤ a then a :: b :: l else b :: ordered_insert l
+
+@[simp] def insertion_sort : list ℕ → list ℕ
+| []       := []
+| (b :: l) := ordered_insert b (insertion_sort l)
+
+end list
