list_extra.lean
@@ -1,10 +1,10 @@
 import .definitions
+import .nat_extra
 
 namespace list
 
 /-
-We're going to need a lot more stuff about lists to prove FTA.
-But for now we just need these (to prove existence).
+Basic lemmas concerning products and prime lists
 -/
 
 lemma product_concat (l1 l2 : list ℕ) : product (l1 ++ l2) = (product l1) * (product l2) :=
@@ -21,6 +21,223 @@ induction l1,
 { from λ h1 : plist (a :: a_1), λ h2 : plist l2, and.intro 
     (and.elim_left h1) 
     (ih_1 (and.elim_right h1) h2)
+}
+end
+
+lemma lmax_head {x y : ℕ} {t : list ℕ} (h : sorted (x :: y :: t)) : y ≤ x := 
+begin
+  simp [sorted] at h,
+  have : max x (lmax (y :: t)) = x, from sorry, -- to_bool issues
+  have hx : max y (lmax t) ≤ x, by rw [←this]; exact le_max_right x (lmax (y :: t)),
+  have hy : y ≤ max y (lmax t), by simp [le_max_left],
+  exact nat.le_trans hy hx
+end
+
+lemma plist_prod_nonzero {l : list ℕ} (h : plist l) : product l ≠ 0 :=
+begin
+  induction l with p t ih,
+  { simp [product] },
+  { simp [product],
+    have ht : plist t, by simp [plist] at h; exact h.right,
+    by_cases p = 0 with hp,
+    { simp [plist, number_theory.irreducible] at h, exact absurd hp h.right.right.left },
+    { have hpg0 : product t ≠ 0, from ih ht,
+      --this was incredibly annoying; any ideas how we could make this easier?
+      have hp : nat.succ (nat.pred p) = p, from nat.succ_pred_eq_of_pos (nat.pos_of_ne_zero hp),
+      have ht : nat.succ (nat.pred (product t)) = product t, from nat.succ_pred_eq_of_pos (nat.pos_of_ne_zero hpg0),
+      have : p*(product t) = 1 + (nat.pred p) + (nat.pred (product t)) + (nat.pred p)*(nat.pred (product t)),
+        by rw [←hp,←ht]; apply nat.foil,
+      have : p*(product t) = nat.succ((nat.pred p) + (nat.pred (product t)) + (nat.pred p)*(nat.pred (product t))),
+        by rw [←nat.one_add]; simp [this],
+      rw [this], exact nat.succ_ne_zero ((nat.pred p) + (nat.pred (product t)) + (nat.pred p)*(nat.pred (product t)))
+    }
+  }
+end
+
+lemma plist_prod_one {l : list ℕ} (h : plist l) : product l = 1 → l = [] :=
+begin
+  cases l with p t,
+  { simp },
+  { intro, simp [product] at a,
+    have : p = 1, from (nat.unique_unit a).left,
+    simp [plist] at h,
+    have : p ≠ 1, from h.left.right.left,
+    contradiction
+  }
+end
+
+/-
+We'll need some machinery about permutations to talk about unique prime lists.
+This stuff is ripped from mathlib.
+-/
+
+variable {α : Type}
+open perm
+
+@[refl] protected theorem perm.refl : ∀ (l : list α), l ~ l
+| []      := perm.nil
+| (x::xs) := skip x (perm.refl xs)
+
+@[symm] protected theorem perm.symm {l₁ l₂ : list α} (p : l₁ ~ l₂) : l₂ ~ l₁ :=
+perm.rec_on p
+  perm.nil
+  (λ x l₁ l₂ p₁ r₁, skip x r₁)
+  (λ x y l, swap y x l)
+  (λ l₁ l₂ l₃ p₁ p₂ r₁ r₂, trans r₂ r₁)
+
+attribute [trans] perm.trans
+
+/-
+Interactions of permutations with our other list definitions
+-/
+
+lemma perm_product {l₁ l₂ : list ℕ} (h : l₁ ~ l₂) : product l₁ = product l₂ :=
+begin
+induction h,
+{ simp },
+{ simp [product,ih_1] },
+{ simp [product] },
+{ simp [ih_1,ih_2] }
+end
+
+lemma perm_lmax {l₁ l₂ : list ℕ} (h : l₁ ~ l₂) : lmax l₁ = lmax l₂ :=
+begin
+induction h,
+{ simp },
+{ simp [lmax,ih_1] },
+{ simp [lmax,max_left_comm] },
+{ simp [ih_1,ih_2] }
+end
+
+lemma perm_plist {l₁ l₂ : list ℕ} (h : l₁ ~ l₂) (hp : plist l₁) : plist l₂ :=
+begin
+-- is there a way to clean up this induction re: term introduction?
+-- check out perm_induction_on in perm.lean in mathlib?
+induction h with x l₁ l₂ l₃ ih x y l l₁ l₂,
+{ exact hp },
+{ have : plist l₁, by simp [plist] at hp; exact hp.right,
+  have hp2 : plist l₂, by simp [this] at ih; exact ih,
+  have : number_theory.irreducible x, by simp [plist] at hp; exact hp.left,
+  by constructor; assumption
+},
+{ have hpx : number_theory.irreducible x, by simp [plist] at hp; exact hp.left,
+  have hpy : number_theory.irreducible y, by simp [plist,plist] at hp; exact hp.right.left,
+  have hpl : plist l, by simp [plist, plist] at hp; exact hp.right.right,
+  have hpyl : plist (y :: l), by constructor; assumption,
+  by constructor; assumption
+},
+{ apply ih_2, apply ih_1, assumption }
+end
+
+/-
+We need to prove the existence of sorted lists. To do this, we introduce a
+sorting algorithm and show that it spits out a sorted permutation.
+-/
+
+lemma perm_ordered_insert (x : ℕ) (l : list ℕ) : ordered_insert x l ~ x :: l :=
+begin
+induction l with y l ih,
+{ simp [ordered_insert] },
+{ by_cases y ≤ x with h,
+  { simp [ordered_insert, h] },
+  { simp [ordered_insert, h],
+    have hxy : y :: x :: l ~ x :: y :: l, by simp [perm.swap],
+    suffices : y :: ordered_insert x l ~ y :: x :: l,
+    { transitivity, apply this, apply hxy },
+    { apply perm.skip, simp [ih] }
+  }
+}
+end
+
+lemma perm_insertion_sort (l : list ℕ) : insertion_sort l ~ l :=
+begin
+induction l with y l ih,
+{ simp [insertion_sort] },
+{ simp [insertion_sort],
+  have h : ordered_insert y (insertion_sort l) ~ y :: insertion_sort l,
+    by apply perm_ordered_insert,
+  transitivity, assumption, apply perm.skip, apply ih
+}
+end
+
+lemma sorted_singleton (x : ℕ) : sorted [x] = tt :=
+begin
+  simp [sorted, lmax, max],
+  by_cases x ≤ 0,
+  { simp [nat.eq_zero_of_le_zero h], from sorry }, -- to_bool issues
+  { simp [h], from sorry } -- to_bool issues
+end
+
+lemma sorted_head (x : ℕ) (l : list ℕ) 
+  : sorted (x :: l) = tt ↔ lmax l ≤ x ∧ sorted l :=
+begin
+split,
+{ intro h, simp [sorted] at h,
+  have hx : max x (lmax l) = x, from sorry, -- to_bool issues
+  split,
+  { rw [←hx], simp [le_max_right] },
+  { from sorry } -- to_bool issues
+},
+{ intro h, simp [sorted],
+  have : max x (lmax l) = x, by simp [max_eq_left h.left],
+  from sorry -- to_bool issues
+}  
+end
+
+lemma sorted_ordered_insert {x : ℕ} {l : list ℕ}
+ : sorted l = tt → sorted (ordered_insert x l) = tt :=
+begin
+intro h, induction l with y l ih,
+{ simp [sorted_singleton] },
+{ by_cases y ≤ x with hxy,
+  { simp [hxy], rw [sorted], admit },
+  { have : x ≤ y ∨ y ≤ x, from le_total x y,
+    have hyx : x ≤ y, by simp [hxy] at this; assumption,
+    have hyl : lmax l ≤ y, by simp [sorted_head] at h; exact h.right,
+    have : ordered_insert x l ~ x :: l, by simp [perm_ordered_insert],
+    have hyxl : lmax (ordered_insert x l) ≤ y, by 
+      simp [perm_lmax this, lmax]; simp [max_le hyx hyl],
+
+    have : sorted l = tt, by
+    begin
+      simp [sorted] at h,
+      from sorry -- to_bool issues
+    end,
+    have hxl : sorted (ordered_insert x l) = tt, from ih this,
+    
+    simp [hxy,sorted_head], apply and.intro,
+    { exact hxl },
+    { exact hyxl }
+  }
+}
+end
+
+lemma sorted_insertion_sort (l : list ℕ) : (sorted $ insertion_sort l) = tt :=
+begin
+induction l with x l ih,
+{ simp [insertion_sort, sorted] },
+{ simp [sorted_ordered_insert ih] }
+end
+
+/-
+Sorting a sorted list is idempotent: idem_insertion_sort. 
+
+We conceptually might want the following lemma:
+
+lemma perm_sorted {l₁ l₂ : list ℕ} (h : l₁ ~ l₂) (hs1 : sorted l₁) (hs2 : sorted l₂) : l₁ = l₂
+
+But this seems very hard to prove given our definition of perm_sorted. So
+instead we'll get the needed result from less general principles.
+-/
+
+lemma idem_insertion_sort {l : list ℕ} (h : sorted l) : insertion_sort l = l :=
+--perm_sorted (perm_insertion_sort l) (sorted_insertion_sort l) h
+begin
+induction l with x t ih,
+{ simp },
+{ have : sorted t = tt, by simp [sorted] at h; from sorry, -- to_bool issues
+  simp [insertion_sort], rw [ih this],
+  induction t, { simp }, { simp [ordered_insert, list.lmax_head h] }
 }
 end
 
