nat_extra.lean
@@ -27,11 +27,6 @@ have m = nat.succ n ∨ m < nat.succ n, from nat.eq_or_lt_of_le hle,
 have m < nat.succ n, from or.resolve_left this hne,
 nat.le_of_lt_succ this
 
-lemma eq_or_less (n : ℕ) : n < 1 → n = 0 :=
-assume h : n < 1,
-have h1 : n+1 ≤ 0+1, from h,
-nat.eq_zero_of_le_zero (le_of_add_le_add_right h1)
-
 lemma lt_imp_ne {m n : ℕ} (h : m < n) : m ≠ n :=
 assume h' : m = n, 
 have hn : n < n, by simp [h'] at h; assumption,
@@ -44,6 +39,11 @@ begin
   existsi n, reflexivity
 end
 
+lemma foil (m n : ℕ) : (nat.succ m)*(nat.succ n) = 1 + m + n + m*n := 
+calc (nat.succ m)*(nat.succ n) = (1+m)*(1+n) : by rw [←nat.one_add m, ←nat.one_add n]
+           ... = 1 * 1 + m * 1 + (1 + m) * n : by rw [left_distrib, right_distrib]
+           ... = 1 + m + n + m*n             : by rw [one_mul, mul_one, right_distrib]; simp
+
 lemma no_zero_divisors {m n : ℕ} : m*n ≠ 0 → m ≠ 0 ∧ n ≠ 0 :=
 assume hmn : m*n ≠ 0,
 have (m = 0 ∨ n = 0) → m*n = 0, from
@@ -52,5 +52,25 @@ have (m = 0 ∨ n = 0) → m*n = 0, from
     (assume hn : n = 0, (eq.symm hn) ▸ mul_zero m),
 have ¬(m = 0 ∨ n = 0), from (mt this) hmn,
 (iff.elim_left (demorgan (m=0) (n=0))) this
+
+lemma unique_unit {m n : ℕ} (H : m*n = 1) : m = 1 ∧ n = 1 :=
+begin revert m, induction n with n ih,
+{ intros; contradiction },
+{ intro m, intro H; cases m with m,
+  { have h01 : 0 = 1, by rw [←H]; simp, contradiction },
+  { have h : 1 + 0 = 1 + (m + n + m*n), from
+    calc 1 + 0 = 1                            : rfl
+           ... = (nat.succ m) * (nat.succ n)  : by rw [←H]
+           ... = 1 + (m + n + m*n)            : by rw [nat.foil]; simp,
+    have hz : m + (n + m*n) = 0, by simp [nat.add_left_cancel h],
+    from and.intro
+      (have hmz: m = 0, from nat.eq_zero_of_add_eq_zero_right hz,
+       show nat.succ m = 1, by rw [hmz])
+      (have hmnz: n + m * n = 0, from nat.eq_zero_of_add_eq_zero_left hz,
+       have hnz: n = 0, from nat.eq_zero_of_add_eq_zero_right hmnz,
+       show nat.succ n = 1, by rw [hnz])
+  }
+}
+end
 
 end nat
